AP/AP/Defense/Box.lean
@@ -1,0 +1,11 @@
+import AP.AP.Defense.Corner
+
+namespace AP.Box
+
+def offset : ℕ := 106
+
+def corners : List Corner :=
+  Dir.univList.map (⟨·, offset⟩)
+
+def defense : Defense :=
+  .ofList # corners.map (·.defense)
